tweaks

paxos/proof.dfy
@@ -130,7 +130,7 @@ predicate Agreement_Inv(c:Constants, ds:DistrSys)
     && ds.WF(c)
     && Agreement(c, ds)
     && LdrBallotNotBottom(c, ds)
-    && FutureBallotsDecisionsProperty(c, ds)
+    && Agreement_Inv_Lemma(c, ds)
 }
 
 
@@ -155,6 +155,7 @@ lemma NextPreservesAgreementInv(c:Constants, ds:DistrSys, ds':DistrSys)
     requires Next(c, ds, ds')
     ensures Agreement_Inv(c, ds')
 {
+
     if exists v, b, i :: c.ValidLdrIdx(i) && LeaderIdxDecidedV(c, ds, i, v, b) {
         // If someone has decided in ds
         NextPreservesAgreementInv_Case_ExistingDecision(c, ds, ds');
@@ -170,6 +171,7 @@ lemma NextPreservesAgreementInv_Case_ExistingDecision(c:Constants, ds:DistrSys, 
     requires exists v, b, i :: c.ValidLdrIdx(i) && LeaderIdxDecidedV(c, ds, i, v, b)
     ensures Agreement_Inv(c, ds')
 {
+    NextPreservesAgreementInvLemma(c, ds, ds');
     var v, b, i :| c.ValidLdrIdx(i) && LeaderIdxDecidedV(c, ds, i, v, b);
     var actor, recvIos:seq<Packet>, sendIos:seq<Packet> :| PaxosNextOneAgent(c, ds, ds', actor, recvIos, sendIos);
     if actor.agt.Ldr? {
@@ -180,7 +182,6 @@ lemma NextPreservesAgreementInv_Case_ExistingDecision(c:Constants, ds:DistrSys, 
                 var b', v' := l.ballot, l.val;
                 if v' != v {
                     assert LeaderIdxDecidedV(c, ds', actor.idx, v', b'); 
-                    lemma_FutureBallotsDecisionsProperty(c, ds, ds');
                     assert LeaderIdxDecidedV(c, ds', i, v, b); 
                     assert false;
                 }
@@ -210,6 +211,15 @@ lemma NextPreservesAgreementInv_Case_NoExistingDecision(c:Constants, ds:DistrSys
 
 ///////////////////////          Agreement Sub-Lemma         /////////////////////////////
 
+
+predicate Agreement_Inv_Lemma(c:Constants, ds:DistrSys) 
+{
+    && c.WF()
+    && ds.WF(c)
+    && FutureBallotsDecisionsProperty(c, ds)
+}
+
+
 /* Assumption that if v is decided with ballot b, then all values decided with ballots
 * b' >= b must be of v */
 predicate FutureBallotsDecisionsProperty(c:Constants, ds:DistrSys)
@@ -225,11 +235,10 @@ predicate FutureBallotsDecisionsProperty(c:Constants, ds:DistrSys)
 }
 
 
-lemma lemma_FutureBallotsDecisionsProperty(c:Constants, ds:DistrSys, ds':DistrSys)
-    requires c.WF() && ds.WF(c)
-    requires FutureBallotsDecisionsProperty(c, ds)
+lemma NextPreservesAgreementInvLemma(c:Constants, ds:DistrSys, ds':DistrSys) 
+    requires Agreement_Inv_Lemma(c, ds)
     requires Next(c, ds, ds')
-    ensures FutureBallotsDecisionsProperty(c, ds');
+    ensures Agreement_Inv_Lemma(c, ds')
 {
     assume false;
 }
